fooScript.sml
@@ -1,5 +1,3 @@
-(* Proof of transitivity of the sublist relationship:*)
-
 open HolKernel Parse boolLib bossLib
 
 val _ = new_theory "foo"
@@ -79,125 +77,30 @@ val sublist_refl = store_thm("sublist_refl",
 Induct_on `l`
 THEN SRW_TAC[][]
 );
+
+val sublist_subset = store_thm("sublist_subset",
+``!l1 l2. sublist l1 l2
+      	  ==> set l1 SUBSET set l2``,
+cheat
+);
+
+
+val sublist_append = store_thm("sublist_append",
+``!l1 l1' l2 l2'. sublist l1 l1' /\ sublist l2 l2'
+      	     	  ==> sublist (l1 ++ l2) (l1' ++ l2')``,
+cheat
+);
+
+
+val sublist_length = store_thm("sublist_length",
+``!l l'. sublist l l' 
+      	     	  ==> LENGTH (l) <= LENGTH(l')``,
+cheat
+);
+
+val sublist_filter = store_thm("sublist_filter",
+``!l. sublist (FILTER P l) l``,
+cheat
+);
+
 val _ = export_theory()
-
-
-
-
-(*
-g `!l1 l2 l3. sublist l1 l2 /\ sublist l2 l3 ==> sublist l1 l3`;
-expand (Induct_on `l1`);
-
-
-For proving the base case
-
-     expand(REPEAT STRIP_TAC);
-expand(SRW_TAC [][]);
-
-    
-
-
-To prove the inductive case
-Induct on l2
-expand(Induct_on `l2`);
-
-
-To prove l2 base case
-expand(REPEAT GEN_TAC);
-expand(SRW_TAC [] []);
-
-
-And then to prove the general inductive case
-Induct on l3
-expand(Induct_on `l3`);
-
-
-
-Proving the base case
-expand(REPEAT GEN_TAC);
-expand(SRW_TAC [] []);
-
-Going back to the main inductive case
-expand(REPEAT GEN_TAC);
-expand(REPEAT STRIP_TAC);
-
-expand(Q_TAC SUFF_TAC `( (h''=h') /\ sublist l1 l2) \/ sublist (h''::l1) l2 `);
-expand(REPEAT STRIP_TAC);
-
-expand(Q_TAC SUFF_TAC `( (h'=h) /\ sublist l2 l3) \/ sublist (h'::l2) l3 `);
-expand(REPEAT STRIP_TAC);
-expand(SRW_TAC [] []);
-expand(METIS_TAC [sublist_def]);
-
-expand(SRW_TAC [] []);
-expand(METIS_TAC [sublist_def]);
-
-expand(SRW_TAC [] []);
-expand(METIS_TAC [sublist_def] );
-
-expand(SRW_TAC [] []);
-expand(METIS_TAC [sublist_def] );
-
-expand(SRW_TAC [] []);
-expand(METIS_TAC [sublist_def] );
-
-
-
-------------------------------------------------------------------------------
-Proof of concatenation respect:
-
-val sublist_def = Define`
-    		  (sublist [] l1 = T) /\
-  (sublist (h::t) [] = F) /\
-  (sublist (x::l1) (y::l2) = (x = y) /\ sublist l1 l2 \/ sublist (x::l1) l2)`;
-
-
-This is to make the sublist theory usable by SRW_TAC
-val _ = export_rewrites ["sublist_def"];
-g `!l1 l2 l3 l4. sublist l1 l3 /\ sublist l2 l4 ==> sublist (APPEND l1 l2) (APPEND l3 l4)`;
-expand (Induct_on `l1`);
-expand (Induct_on `l2`);
-
-to prove the base case;
-expand(SRW_TAC [] []);
-expand (Induct_on `l3`);
-
-to prove the base case
-expand(SRW_TAC [] []);
-expand (Induct_on `l4`);
-
-to prove the base case
-expand(SRW_TAC [] []);
-expand (Induct_on `l3`);
-expand(SRW_TAC [] []);
-
-To prove l4 inductive case:
-expand(REPEAT STRIP_TAC);
-expand(FULL_`SIMP_TAC (srw_ss()) []);
-
-
-repeating the same to prove the inductive step of l1
-expand (Induct_on `l2`);
-expand (Induct_on `l3`);
-expand(SRW_TAC [] []);
-expand (Induct_on `l4`);
-expand(SRW_TAC [] []);
-expand(REPEAT STRIP_TAC);
-expand(SRW_TAC [][]);
-expand(Q_TAC SUFF_TAC `( (h''=h') /\ sublist l1 l3) \/ sublist (h''::l1) l3 `);
-expand(REPEAT STRIP_TAC);
-expand(METIS_TAC [sublist_def, listTheory.APPEND_NIL]);
-expand(METIS_TAC [sublist_def, listTheory.APPEND_NIL]);
-expand(METIS_TAC [sublist_def]);
-
-
-repeating the same to prove the inductive step of l2
-expand (Induct_on `l3`);
-expand (Induct_on `l4`);
-expand(SRW_TAC [][]);
-expand(FULL_SIMP_TAC (srw_ss()) []);
-expand(REPEAT STRIP_TAC);
-expand(FULL_SIMP_TAC (srw_ss()) []);
-
-
-*)
